examples/knot/Knot1.v
@@ -108,7 +108,7 @@ Section KNOT.
     Definition SKnotSem: SModSem.t := {|
       SModSem.fnsems := KnotSbtb;
       SModSem.mn := "Knot";
-      SModSem.initial_mr := (GRA.embed (var_points_to sk "_f" Vundef)) ⋅ (GRA.embed (knot_full None)) ;
+      SModSem.initial_mr := (GRA.embed (var_points_to sk "_f" (Vint 0))) ⋅ (GRA.embed (knot_full None)) ;
       SModSem.initial_st := tt↑;
     |}
     .
