examples/new_echo/NewEchoAll.v
@@ -8,44 +8,19 @@ Set Implicit Arguments.
 
 
 
-(* Definition _point_wise_wf: *)
-(*   forall (Ml: list URA.t) (x: GRA.of_list Ml) (n: nat), Prop. *)
-(* Proof. *)
-(*   fix IH 1. *)
-
-(* as IH. *)
-
-(* Fixpoint _point_wise_wf (Ml: list URA.t) (x: GRA.of_list MS) (n: nat): Prop := *)
-(*   match Ml with *)
-(*   | [] => True *)
-(*   | Mhd::Mtl => *)
-(*     @URA.wf Mhd (GRA.of_list *)
-
-(*     point_wise_wf Mtl *)
-
-(* Lemma GRA_of_list_point_wise_wf *)
-(*       (MS: list URA.t) (x: GRA.of_list MS) *)
-(*       (forall n, *)
-
-
-(*   : *)
-(*     URA.wf x. *)
-(* Proof. *)
-(* Admitted. *)
-
 Definition EchoGRA: GRA.t := GRA.of_list [Mem1.memRA; stkRA].
 Local Existing Instance EchoGRA.
 
 Instance memRA_inG: @GRA.inG Mem1.memRA EchoGRA.
 Proof.
   exists 0. ss. Show Proof.
-Qed.
+Defined.
 Local Existing Instance memRA_inG.
 
 Instance stkRA_inG: @GRA.inG stkRA EchoGRA.
 Proof.
   exists 1. ss.
-Qed.
+Defined.
 Local Existing Instance stkRA_inG.
 
 
@@ -121,7 +96,7 @@ Section PROOF.
     etrans.
     { rewrite Mod.add_list_app. eapply refines_proper_r.
       eapply adequacy_open. i. exists ε. split.
-      { admit "URA wf". }
+      { g_wf_tac; repeat (i; splits; ur; ss). refl. }
       { ii. ss. }
     }
     pose (kmd1 := [NewStack3A.KStack; KEcho]).
@@ -142,7 +117,7 @@ Section PROOF.
     transitivity (KMod.transl_src_list kmd1 ++ [Main; Client]); [|refl].
     eapply refines2_app; [|refl].
     eapply adequacy_open. i. exists ε. split.
-    { admit "URA wf". }
+    { g_wf_tac; repeat (i; splits; ur; ss). refl. }
     { ii. ss. }
   Qed.
 End PROOF.
